LeanProjeto2/ShoenfieldsFunctInterp.lean
@@ -1,4 +1,9 @@
---import LeanProjeto2.StarLang_old
+import LeanProjeto2.FOL
+import LeanProjeto2.StarLang
+import MathLib.Tactic
+
+open FOL
+open LFormula
 
 --open StarLang
 --open FType
@@ -18,19 +23,47 @@ def SH_int : Formula → Formula
 
 def SH_int : Formula → Formula                              LISTAS DE VAR UNIV E VAR EXIST? List Term → List Term → Formula → Formula
 | SH_base
-    | isBase A => A
+    | (isBase A) => A
 | V a E b A_ , V c E d B_ => V a V c E b E d (A_ ∨₁ B_)
     | {a} {b} A_ , c d B_ => {a c} {b d} (A_ ∨₁ B_)         USAR APPEND DAS LISTAS?
 | SH_not
     | {a} {b} A_ =>                                         COMO CRIAR f a partir de b e a' a partir de a???
+                                                            acho que precisamos de usar substitution
 | SH_unb_forall
 | SH_b_forall
 
--/
+def interp : Formula → Formula
+| SH_base: (isBase A) => A
 
 
-/-
-def pi_app_transform2 : Term → Term
-| (Π₁·q)·_ => q   -- Transform (Π₁·q)·_ to q
-| t => t
+
+def shoenfield_interpretation : Formula → Formula
+| Formula.lcons p ts => Formula.lcons p ts
+| Formula.not A =>
+  Formula.forall_L "f" (Formula.exists_L "a'" (Formula.not_L (subst_formula "a" (LTerm.Lfunc "f" [LTerm.Lvar "a"]) (shoenfield_interpretation A))))
+| Formula.or A B =>
+  let A_SH := shoenfield_interpretation A in
+  let B_SH := shoenfield_interpretation B in
+  Formula.forall_L "a" (Formula.exists_L "b" (subst_formula "a" (LTerm.Lvar "b") A_SH)) ∧
+  Formula.forall_L "c" (Formula.exists_L "d" (subst_formula "c" (LTerm.Lvar "d") B_SH)) →
+  Formula.forall_L "a" (Formula.forall_L "c" (Formula.exists_L "b" (Formula.exists_L "d" (Formula.or_L (subst_formula "a" (LTerm.Lvar "b") A_SH) (subst_formula "c" (LTerm.Lvar "d") B_SH)))))
+| Formula.bForall x A =>
+  let A_SH := shoenfield_interpretation A in
+  Formula.forall_L x (Formula.forall_L "a" (Formula.exists_L "b" (subst_formula x (LTerm.Lvar "a") A_SH)))
+| Formula.exists_L x A =>
+  let A_SH := shoenfield_interpretation A in
+  Formula.forall_L "a" (Formula.exists_L "b" (Formula.exists_L x (subst_formula x (LTerm.Lvar "a") A_SH)))
+| Formula.bounded_forall_L x t A =>
+  let A_SH := shoenfield_interpretation A in
+  Formula.forall_L "a" (Formula.exists_L "b" (Formula.forall_L x (Formula.and_L (Formula.atomic_L "in" [LTerm.Lvar x, t]) (subst_formula x (LTerm.Lvar "a") A_SH))))
+
+--inductive SHint : Finset String → Finset String → Formula → Formula
+--| sorry
+
+
 -/
+
+--inductive shoenfield_interpretation : Formula → Formula
+--| SH_base (h: isBase A) A : shoenfield_interpretation
+
+--def SH_int (α β : Finset String) (A : Formula) : Formula := ∀ α, ∃ β
